MetaTools/MetaTools.Erase.fst
@@ -1,0 +1,106 @@
+module MetaTools.Erase
+
+open MetaTools.BrowseTerm
+open MetaTools.NamesOfTerm
+
+module U = MetaTools.Util
+module L = FStar.List.Tot
+
+open FStar.Tactics
+
+let typechecks (t: term): Tac bool
+  = Some? (trytac (fun _ -> tc (top_env ()) t))
+
+
+type label =
+type labeled (a: Type) =
+
+assume val placeholder: (#a: Type) -> a
+
+let erase #a (v: labeled a) (at: label): labeled a
+  = placeholder
+
+let erase_term_helper
+  (eraseVarParam: term)
+  (rebuildToplevel: term -> Tac term)
+  (t: term)
+  = let erased_t = pack (Tv_App (`erase) (t, Q_Explicit)) in
+    if typechecks erased_t
+    then erased_t
+    else t
+
+let erase_term (eraseVarParam t: term): Tac term = 
+  fst
+  (browse_term #unit
+    (fun beforeTransform rebuildToplevel boundedVariables parents currentTerm -> 
+      ( if beforeTransform
+        then erase_term_helper eraseVarParam rebuildToplevel currentTerm
+        else currentTerm
+      ), ()
+    )
+    t)
+
+
+let blacklist_lioCore (n: name) =
+  match n with
+  | "FStar"::_
+  | "List"::_
+  | "LowStar"::_
+  | "Prims"::_ -> true
+  | _ -> false
+
+let bv_erase = "cur_label_name_GLOBAL"
+
+open FStar.Tactics.Typeclasses
+
+
+let replace_fv (t: term) (r: list (name * name))
+  : Tac term
+  = fst (browse_term #unit begin
+    fun beforeTransform _ _ _ currentTerm
+    -> ( if beforeTransform
+        then begin
+             match inspect currentTerm with
+             | Tv_FVar fv ->
+               let n = inspect_fv fv in
+               ( match L.find (fun (old, _) -> old = n) r with
+               | Some (_, newName) -> pack (Tv_FVar (pack_fv newName))
+               | _ -> currentTerm
+               )
+             | _ -> currentTerm
+             end
+        else currentTerm ), ()
+  end t)
+
+let make_erased_name (n: name): Tac name =
+  cur_module () @ [last n ^ "_erased"]
+
+let make_erased_names (n: list name): Tac (list (_ * _))
+  = map (fun n -> n, make_erased_name n) n
+
+let erase_term_and_defs (def: term)
+  =
+    let label_var: bv = pack_bv ({
+        bv_ppname = bv_erase;
+        bv_sort = `label;
+        bv_index = 0;
+    }) in
+    let label_var_term = pack (Tv_Var label_var) in 
+    let g: graph = fv_dependencies_of
+    (             blacklist_ulib
+      `join_pred` blacklist_uu
+      `join_pred` blacklist_lioCore) def
+    in
+    let h arg: Tac (option (term * term)) =
+      let toplevel_name, dependencies = arg in
+      let replacements = make_erased_names dependencies in
+      let patch t: Tac term = replace_fv t replacements in
+      U.optmap (fun (typ, def)
+        -> 
+          let b_lvar = fresh_binder (`label) in
+          mk_tot_arr [b_lvar] (patch (erase_term (binder_to_term b_lvar) typ))
+        , mk_abs [pack_binder label_var Q_Explicit] (patch (erase_term label_var_term def))
+      ) (U.sglet_of_name toplevel_name)
+    in
+    map h g
+    
