MetaTools/MetaTools.NamesOfTerm.fst
@@ -1,0 +1,139 @@
+module MetaTools.NamesOfTerm
+
+open FStar.Tactics
+open Control.Monoid
+
+open FStar.Tactics.Typeclasses
+open MetaTools.Util
+open MetaTools.BrowseTerm
+
+module L = FStar.List.Tot
+
+
+// browseFun s = bool -> (term -> Tac term) -> list bv -> list term_view_head -> term -> Tac (term * s)
+let browse_term (#s: Type0) [| monoid s |]
+  (f: browseFun s)
+  (t: term)
+  : Tac (term * s) = browse_term' f id [] [] t
+
+
+let rec names_of_pattern (p: pattern): list name =
+  match p with
+  | Pat_Cons   x l ->
+    let f (v: pattern * bool) = names_of_pattern (admit (); fst v) in
+    let l = L.map f l in
+    L.fold_left (@) [inspect_fv x] l
+  | _ -> []
+
+let rec (@!) (#a: eqtype) (l1 l2: list a)
+  : Tot (list a) (decreases l2) = 
+  match l2 with
+  | [] -> l1
+  | hd::tl -> if L.mem hd l1
+            then l1 @! tl
+            else (hd::l1) @! tl
+
+let fvsOfTerm_helper (t: term_view)
+  : Tac (list name)
+  = match t with
+  | Tv_FVar  fv-> [inspect_fv fv]
+  | Tv_Match _ branches ->
+      L.fold_left (@!) [] (
+        L.map (fun (pat, _) -> names_of_pattern pat) branches
+      )
+  | _ -> []
+
+open Control.Semigroup
+
+let lsetSemiGroup (#a: eqtype) : semigroup (list a)
+  = mkSemigroup _ (@!)
+
+let lsetIsMonoid (#a: eqtype) : monoid (list a) = 
+  mkMonoid _ #lsetSemiGroup []
+
+let fvsOfTerm (t: term)
+  : Tac (list name)
+  = snd (browse_term #_ #lsetIsMonoid begin
+    fun beforeTransform _ _ _ currentTerm
+    -> currentTerm,
+      ( if beforeTransform
+        then fvsOfTerm_helper currentTerm
+        else [] )
+  end t)
+
+
+unfold let graph = list (name * list name) 
+let g_get (g: graph) k = L.find (fun (n, _) -> n = k) g
+let g_mem (g: graph) k = Some? (g_get g k)
+let g_rm (g: graph) k: graph =
+  L.filter (fun (n, _) -> false = (n = k)) g
+let g_set (g: graph) k v = (k, v)::g_rm g k
+let g_values (g: graph): list name =
+  mconcat #_ #lsetIsMonoid (L.map snd g)
+
+unfold let negPred f x = false = f x 
+
+let g_get_unexplored_names (g: graph): list name
+  = let vals = g_values g in
+    L.filter (negPred (g_mem g)) vals
+
+let isGraphComplete (g: graph): bool
+  = Nil? (g_get_unexplored_names g)
+
+let g_resolve_once (filterNames: name -> bool) (g: graph): Tac (graph * done: bool)
+  = let l = g_get_unexplored_names g in
+    fold_left #graph begin
+      fun g n -> 
+        let deps = match sglet_of_name n with
+        | Some (typ, def) -> 
+          fvsOfTerm typ @! fvsOfTerm def
+        | None            -> [] in
+        g_set g n (L.filter (negPred filterNames) deps)        
+    end g l, Nil? l
+
+let rec g_resolve (filterNames: name -> bool) (g: graph): Tac graph
+  = let g, continue = g_resolve_once filterNames g in
+    if continue
+    then g_resolve filterNames g
+    else g
+
+let g_sort_helper (a b: name * list name)
+  = let (a, a_deps), (b, b_deps) = a, b in
+    if L.mem a b_deps
+    then  1
+    else begin
+      if L.mem b a_deps
+      then -1
+      else 0
+    end
+let g_sort g = L.sortWith g_sort_helper g
+
+let rootName = ["{root}"]
+
+let fv_dependencies_of (filterNames: name -> bool) (t: term)
+  : Tac graph
+  = let deps = L.filter (negPred filterNames) (fvsOfTerm t) in 
+    let g = g_set [] rootName deps in
+    let g = g_sort (g_resolve filterNames g) in
+    g
+
+[@plugin]
+let fv_dependencies_of' (blacklist: list name) (t: term): Tac graph
+  = fv_dependencies_of (fun n -> L.mem n blacklist) t
+
+let join_pred (p: 'a -> bool) (q: 'a -> bool) (v: 'a): bool
+  = p v || q v
+
+let blacklist_uu (n: name) =
+  match n with
+  | [] -> false
+  | _ ->  prefixOfStr "uu_" (last n)
+ 
+let blacklist_ulib (n: name) =
+  match n with
+  | "FStar"::_
+  | "List"::_
+  | "LowStar"::_
+  | "Prims"::_ -> true
+  | _ -> false
+
