MetaTools/MetaTools.Util.fst
@@ -51,3 +51,91 @@ let term_head t : Tac term_view_head =
   | Tv_AscribedT _ _ _ -> Th_AscribedT
   | Tv_AscribedC _ _ _ -> Th_AscribedC
 
+
+let sglet_of_name (name: name): Tac (option (typ * term)) 
+  = match lookup_typ (top_env ()) name with
+    | Some f -> begin
+      match inspect_sigelt f with
+      | Sg_Let r fv _ typ def -> Some (typ, def)
+      | _ -> None
+      end
+    | None -> None
+
+let rec exists_in_list  (eq: 'a -> 'a -> bool) (v: 'a) (l: list 'a) =
+  match l with
+  | [] -> false
+  | hd::tl -> 
+    if eq hd v then true else exists_in_list eq v tl
+
+let rec rm_dup_in_list_helper #a (eq: a -> a -> bool) (l: list a) (seen: list a)
+    : list a
+    = match l with
+    | [] -> []
+    | hd::tl -> if exists_in_list eq hd seen
+              then rm_dup_in_list_helper eq tl seen
+              else hd::rm_dup_in_list_helper eq tl (hd::seen) 
+
+let rm_dup_in_list (eq: 'a -> 'a -> bool) (l: list 'a) =
+  rm_dup_in_list_helper eq l []
+
+let rec last (l: list 'a {Cons? l}): 'a = 
+  match l with
+  | [hd] -> hd
+  | hd::tl -> last tl
+
+
+let rec names_of_pattern (p: pattern): list name =
+  match p with
+  | Pat_Cons   x l ->
+    let f (v: pattern * bool) = names_of_pattern (admit (); fst v) in
+    let l = L.map f l in
+    L.fold_left (@) [inspect_fv x] l
+  | _ -> []
+
+
+open Control.Monoid
+open FStar.Tactics.Typeclasses
+
+let bindM (#s: Type0) [| monoid s |] #a #b (x: a * s) (f: a -> Tac (b * s)): Tac (b * s) =
+    let result, s0 = x in
+    let result, s1 = f result in
+    result, s0 <+> s1
+
+let optmap #a #b (f: a -> Tac b) (x: option a): Tac (option b)
+  = match x with
+  | Some v -> Some (f v)
+  | None   -> None
+
+let optmapS (#s: Type0) [| monoid s |] #a #b (f: a -> Tac (b * s)) (x: option a): Tac (option b * s)
+  = match optmap f x with
+  | Some (v,s0) -> Some v, s0 
+  | None        -> None  , mempty
+  
+let focusFst ((a,b),c) = a,c
+
+
+
+type sg_Let' =
+       (r:bool)
+  * (  (fv:fv)
+  *  ( (us:list string)
+  *   ((typ:typ)
+  *    (def:term)
+    )))
+
+let dummy_range = range_of "DUMMY_RANGE"
+
+let sg_let'_to_Sg_Let
+  (sglet: sg_Let')
+  = let r, (fv, (us, (typ, def))) = sglet in
+    Sg_Let r fv (L.map (fun x -> dummy_range, x) us) typ def
+
+
+
+let rec prefixOf (#a:eqtype) (prefix l: list a) =
+  match prefix, l with
+  | hdP::tlP, hdL::tlL -> if hdP = hdL then prefixOf tlP tlL else false
+  | [], _ -> true
+  | _ -> false
+let prefixOfStr prefix str = prefixOf (String.list_of_string prefix) (String.list_of_string str)
+
